powerpc/eabi/CPragmas.ml
@@ -35,20 +35,20 @@ let process_section_pragma classname istring ustring addrmode accmode =
 
 let process_use_section_pragma classname id =
   if not (Sections.use_section_for (intern_string id) classname)
-  then C2Clight.error (sprintf "unknown section name `%s'" classname)
+  then C2C.error (sprintf "unknown section name `%s'" classname)
 
 (* #pragma reserve_register *)
 
 let process_reserve_register_pragma name =
   match Machregsaux.register_by_name name with
   | None ->
-      C2Clight.error "unknown register in `reserve_register' pragma"
+      C2C.error "unknown register in `reserve_register' pragma"
   | Some r ->
       if Machregsaux.can_reserve_register r then
         Coloringaux.reserved_registers :=
           r :: !Coloringaux.reserved_registers
       else
-        C2Clight.error "cannot reserve this register (not a callee-save)"
+        C2C.error "cannot reserve this register (not a callee-save)"
 
 (* Parsing of pragmas using regexps *)
 
@@ -87,22 +87,22 @@ let process_pragma name =
       (Str.matched_group 5 name); (* accmode *)
     true
   end else if Str.string_match re_start_pragma_section name 0 then
-    (C2Clight.error "ill-formed `section' pragma"; true)
+    (C2C.error "ill-formed `section' pragma"; true)
  else if Str.string_match re_pragma_use_section name 0 then begin
     let classname = Str.matched_group 1 name
     and idents = Str.matched_group 2 name in
     let identlist = Str.split re_split_idents idents in
-    if identlist = [] then C2Clight.warning "vacuous `use_section' pragma";
+    if identlist = [] then C2C.warning "vacuous `use_section' pragma";
     List.iter (process_use_section_pragma classname) identlist;
     true
   end else if Str.string_match re_start_pragma_use_section name 0 then begin
-    C2Clight.error "ill-formed `use_section' pragma"; true
+    C2C.error "ill-formed `use_section' pragma"; true
   end else if Str.string_match re_pragma_reserve_register name 0 then begin
     process_reserve_register_pragma (Str.matched_group 1 name); true
   end else if Str.string_match re_start_pragma_reserve_register name 0 then begin
-    C2Clight.error "ill-formed `reserve_register' pragma"; true
+    C2C.error "ill-formed `reserve_register' pragma"; true
   end else
     false
 
 let initialize () =
-  C2Clight.process_pragma_hook := process_pragma
+  C2C.process_pragma_hook := process_pragma
