test/regression/annot1.c
@@ -1,0 +1,23 @@
+#include <stdio.h>
+
+/* Annotations */
+
+int f(int x, int y)
+{
+  return __builtin_annotation("f(%1,%2)", x, y);
+}
+
+double g(double x)
+{
+  return __builtin_annotation("g(%1 + 1.0)", x + 1.0);
+}
+
+int main()
+{
+  __builtin_annotation("calling f");
+  printf("f returns %d\n", f(12, 34));
+  __builtin_annotation("calling g");
+  printf("f returns %.2f\n", g(3.14));
+  return 0;
+}
+
